theories_unscoped/MappingOneTwo.v
@@ -1,0 +1,86 @@
+From Equations Require Import Equations.
+From Prototype Require Import Prelude Sig.
+From Prototype Require LevelOne LevelTwo.
+
+Module Make (S : Sig).
+Module O := LevelOne.Make (S).
+Module T := LevelTwo.Make (S).
+
+(*********************************************************************************)
+(** *** Denotation (level two -> level one). *)
+(*********************************************************************************)
+
+Definition denote_type (k : T.kind) : Type :=
+  match k with 
+  | T.Ks => O.subst
+  | T.Km T.Kt => O.expr O.Kt
+  | T.Km (T.Kal tys) => O.expr (O.Kal tys)
+  | T.Km (T.Ka ty) => O.expr (O.Ka ty)
+  end.
+      
+(** Denotation doesn't know how to handle metavariables: it thus works up to an
+    assignment, which determines how to denote metavariables. *)
+Definition assignment := forall k : T.kind, T.mvar k -> denote_type k.
+
+(** Mapping from level two expressions to level one expressions and substitutions. *)
+Equations denote {k} (m : assignment) (t : T.expr k) : denote_type k by struct t :=
+denote m (T.E_var i) := O.E_var i ;
+denote m (T.E_ctor c al) := O.E_ctor c (denote m al) ;
+denote m T.E_al_nil := O.E_al_nil ;
+denote m (T.E_al_cons a al) := O.E_al_cons (denote m a) (denote m al) ;
+denote m (T.E_abase b x) := O.E_abase b x ;
+denote m (T.E_aterm t) := O.E_aterm (denote m t) ;
+denote m (T.E_abind a) := O.E_abind (denote m a) ;
+denote m (@T.E_subst T.Kt t s) := O.substitute (denote m t) (denote m s) ;
+denote m (@T.E_subst (T.Ka _) t s) := O.substitute (denote m t) (denote m s) ;
+denote m (@T.E_subst (T.Kal _) t s) := O.substitute (denote m t) (denote m s) ;
+denote m (T.E_sshift k) := O.sshift k ;
+denote m (T.E_scons t s) := O.scons (denote m t) (denote m s) ;
+denote m (T.E_scomp s1 s2) := O.scomp (denote m s1) (denote m s2) ;
+denote m (T.E_mvar x) := m _ x.
+
+(*********************************************************************************)
+(** *** Correctness of denotation. *)
+(*********************************************************************************)
+
+(** Equality on denoted expressions. We use pointwise equality 
+    for substitutions so as to not assume functional extensionality. *)
+Definition denote_rel (k : T.kind) : relation (denote_type k) :=
+  match k with 
+  | T.Ks => @point_eq nat (O.expr O.Kt)
+  | _ => eq
+  end.
+
+#[global] Instance denote_rel_equiv k : Equivalence (denote_rel k).
+Proof. 
+constructor ; destruct k ; try solve [easy].
+- intros ?????. etransitivity ; eauto.
+- intros ?????. etransitivity ; eauto.
+Qed.
+
+(** Main correctness result for [denote]: it transports level-two _sigma-equal_ terms 
+    to level-one _equal_ terms. *)
+#[global] Instance denote_proper {k} m : Proper (T.axiom_eq ==> denote_rel k) (@denote k m).
+Proof.
+intros t1 t2 Ht. induction Ht ; simpl in * ; simp denote.
+all: try solve [ auto | easy ].
+- etransitivity ; eauto. 
+- destruct k ; simp denote ; now apply O.substitute_proper.
+- now apply O.scons_proper.
+- now apply O.scomp_proper.
+- simp substitute. f_equal. apply O.substitute_proper ; auto.
+  simp up_subst denote. rewrite O.up_subst_alt. reflexivity.
+- destruct k ; simp denote ; now rewrite O.subst_subst.
+- destruct k ; unfold T.sid ; simp denote ; now rewrite O.subst_sid.
+- now rewrite O.sid_scons.
+- unfold T.sid ; simp denote. now rewrite O.scomp_id_r.
+- now rewrite O.scomp_assoc.
+- now rewrite O.scomp_scons_distrib.
+Qed.
+
+(*********************************************************************************)
+(** *** Reification (level one -> level two). *)
+(*********************************************************************************)
+
+
+End Make.
